src/localdrfpf/LocalPFSim.v
@@ -30,8 +30,8 @@ Require Import MemoryProps.
 Require Import OrderedTimes.
 Require SimMemory.
 
-Require Import LocalDRFDef.
-Require Import LocalDRF_PF.
+Require Import LocalPF.
+Require Import LocalPFThread.
 Require Import TimeTraced.
 Require Import PFConsistentStrong.
 Require Import Mapping.
@@ -2334,7 +2334,7 @@ Section SIM.
         (WF_SRC: Configuration.wf c_src0)
         (WF_MID: JConfiguration.wf views0 c_mid0)
         (WF_TGT: Configuration.wf c_tgt0)
-        (RACEFREE: racefree L c_src0)
+        (RACEFREE: pf_racefree L c_src0)
     :
       (<<BEH: forall beh, behaviors (pf_step L) c_src0 beh>>) \/
       (exists s, (<<EVENT: e = MachineEvent.syscall s>>) /\
@@ -2431,7 +2431,7 @@ Section SIM.
     i. des.
 
     dep_inv STEPSRC0.
-    exfalso. eapply racefree_write_read.
+    exfalso. eapply pf_racefree_write_read.
     { eauto. }
     { eapply silent_pf_steps_trace_pf_steps_trace; eauto. }
     { econs 2.
@@ -2449,132 +2449,3 @@ Section SIM.
   Admitted.
 
 End SIM.
-
-
-
-Lemma sim_configuration_beh L times c_src c_mid c_tgt views prom extra
-      (WO: forall loc, well_ordered (times loc))
-      (INCR: forall nat loc, times loc (incr_time_seq nat))
-      (RACEFRFEE: racefree L c_src)
-      (WF_SRC: Configuration.wf c_src)
-      (WF_MID: JConfiguration.wf views c_mid)
-      (WF_TGT: Configuration.wf c_tgt)
-      (SIM: sim_configuration L times (fun _ => True) views prom extra c_src c_mid c_tgt)
-  :
-    behaviors (times_configuration_step_all times) c_tgt <1=
-    behaviors (pf_step L) c_src.
-Proof.
-  i. ginduction PR; i.
-  { dep_inv SIM. econs 1. ii. ss.
-    specialize (THSPF tid). specialize (THSJOIN tid).
-    setoid_rewrite FIND in THSPF. unfold option_rel in *. des_ifs.
-    dep_inv THSPF. dep_inv THSJOIN.
-    eapply TERMINAL in Heq0. des. splits; auto.
-    inv THREAD. inv LOCAL. inv LOCAL0. ss. subst.
-    econs. exploit sim_promise_bot; eauto. eapply Memory.ext.
-    i. specialize (PROMISES0 loc ts). erewrite Memory.bot_get in *.
-    inv PROMISES0; ss. }
-  { inv STEP.
-    destruct (classic (List.Forall
-                         (fun the => no_read_msgs
-                                       (all_promises (fun tid' => tid <> tid') prom)
-                                       (snd the)) (tr ++ tr_cert))).
-    { exploit step_sim_configuration; eauto. i. des. unguard. des; ss. dep_inv STEPSRC.
-      econs 2; eauto.
-      { econs; eauto. }
-      { eapply IHPR; try apply SIM0; eauto.
-        { eapply steps_racefree; eauto. econs; eauto. econs. }
-        { eapply pf_step_trace_future; eauto. }
-        { eapply JConfiguration.step_future; eauto. }
-        { eapply times_configuration_step_future; eauto. }
-      }
-    }
-    { exploit promise_read_race; eauto. i. des; clarify. }
-  }
-  { inv STEP.
-    destruct (classic (List.Forall
-                         (fun the => no_read_msgs
-                                       (all_promises (fun tid' => tid <> tid') prom)
-                                       (snd the)) (tr ++ tr_cert))).
-    { exploit step_sim_configuration; eauto. i. des. unguard. des; ss.
-      { dep_inv STEPSRC. econs 3; eauto. econs; eauto. }
-      { dep_inv STEPSRC. econs 3; eauto. econs; eauto. }
-    }
-    { exploit promise_read_race; eauto. i. des; clarify. }
-  }
-  { inv STEP.
-    destruct (classic (List.Forall
-                         (fun the => no_read_msgs
-                                       (all_promises (fun tid' => tid <> tid') prom)
-                                       (snd the)) (tr ++ tr_cert))).
-    { exploit step_sim_configuration; eauto. i. des. unguard. des; ss. dep_inv STEPSRC.
-      { econs 4; eauto.
-        { econs; eauto. }
-        { eapply IHPR; try apply SIM0; eauto.
-          { eapply steps_racefree; eauto. econs; eauto. econs. }
-          { eapply pf_step_trace_future; eauto. }
-          { eapply JConfiguration.step_future; eauto. }
-          { eapply times_configuration_step_future; eauto. }
-        }
-      }
-      { eapply IHPR; try apply SIM0; eauto.
-        { eapply JConfiguration.step_future; eauto. }
-        { eapply times_configuration_step_future; eauto. }
-      }
-    }
-    { exploit promise_read_race; eauto. i. des; clarify. }
-  }
-Qed.
-
-Theorem local_DRF_PF L s
-        (RACEFRFEE: racefree L (Configuration.init s))
-  :
-    behaviors Configuration.step (Configuration.init s) <1=
-    behaviors (pf_step L) (Configuration.init s).
-Proof.
-  i. eapply times_configuration_step_same_behaviors in PR; cycle 1.
-  { eapply Configuration.init_wf. }
-  des. eapply sim_configuration_beh; eauto.
-  { eapply Configuration.init_wf. }
-  { eapply JConfiguration.init_wf. }
-  { eapply Configuration.init_wf. }
-  instantiate (1:=s). instantiate (1:=bot4). instantiate (1:=bot3). econs; eauto.
-  { i. unfold Threads.init. repeat erewrite IdentMap.Facts.map_o.
-    unfold option_map. des_ifs. ss. econs. econs.
-    econs; ss. i. erewrite Memory.bot_get. destruct (classic (L loc)).
-    { econs 1; eauto. }
-    { econs 2; eauto.  }
-  }
-  { i. unfold Threads.init. repeat erewrite IdentMap.Facts.map_o.
-    unfold option_map. des_ifs. ss. econs. econs.
-    { refl. }
-    { ii. erewrite Memory.bot_get. econs. }
-  }
-  { i. splits; ss. }
-  { econs.
-    { i. unfold Memory.init, Memory.get. erewrite Cell.init_get. des_ifs.
-      { econs 2; eauto.
-        { ii. inv H. ss. }
-        { ii. inv H. ss. }
-        { refl. }
-        { i. apply eq_lb_time. }
-      }
-      { econs.
-        { ii. inv H. ss. }
-        { ii. inv H. ss. }
-      }
-    }
-    { i. inv EXTRA. ss. }
-  }
-  { refl. }
-  { i. unfold JConfiguration.init_views. des_ifs. econs; eauto.
-    eapply Memory.closed_view_bot. eapply Memory.init_closed. }
-  { refl. }
-  { ii. unfold Memory.init, Memory.get in GET. erewrite Cell.init_get in GET.
-    des_ifs. auto. }
-  { i. unfold Threads.init in GET. erewrite IdentMap.Facts.map_o in GET.
-    unfold option_map in GET. des_ifs. dep_clarify. ii. ss. eexists [], _. splits; auto.
-    { refl. }
-    { right. ss. }
-  }
-Qed.
